Launchbury/LaunchburyCombinedTagged.thy
@@ -371,7 +371,7 @@ text {* Evaluation does not touch the tail of the stack. *}
 
 lemma stack_unchanged:
   assumes "\<Gamma> \<Down>\<^sup>i\<^sup>u\<^bsub>S\<^esub> \<Delta>"
-  assumes "distinct S"
+  assumes "x \<noteq> hd S"
   assumes "x \<in> set (tl S)"
   assumes "(x,e) \<in> set \<Gamma>"
   shows   "(x,e) \<in> set \<Delta>"
@@ -379,7 +379,9 @@ using assms
  apply (induct \<Gamma> i u S \<Delta> arbitrary: x e rule:reds.induct)
  apply (auto simp add: perm_set_eq)
   apply (metis fresh_Pair set_not_fresh)
-  apply (metis (mono_tags) fresh_Pair fresh_list_elem not_self_fresh)+
+  apply (metis fresh_PairD(1) fresh_list_elem not_self_fresh)
+  apply metis
+  apply (metis fresh_Pair heapVars_from_set heapVars_not_fresh)
 done
   
 text {* 
